src/fs/super.dfy
@@ -57,7 +57,7 @@ module FsKinds {
     ensures super.Valid()
   {}
 
-  datatype SuperBlock = SuperBlock(info: Super, disk_size: uint64)
+  datatype SuperBlock = SuperBlock(info: Super, actual_blocks: uint64)
   {
     // a random number
     static const magic: uint64 := 0x5211cc92a57dd76b;
@@ -73,7 +73,7 @@ module FsKinds {
       IntEncoding.le_enc64(magic) +
         IntEncoding.le_enc64(info.inode_blocks as uint64) +
         IntEncoding.le_enc64(info.data_bitmaps as uint64) +
-        IntEncoding.le_enc64(disk_size) +
+        IntEncoding.le_enc64(actual_blocks) +
         C.repeat(0 as byte, 4096-(8*4))
     }
 
@@ -86,7 +86,7 @@ module FsKinds {
       IntEncoding.UInt64Put(magic, 0, b);
       IntEncoding.UInt64Put(info.inode_blocks as uint64, 8, b);
       IntEncoding.UInt64Put(info.data_bitmaps as uint64, 16, b);
-      IntEncoding.UInt64Put(disk_size as uint64, 24, b);
+      IntEncoding.UInt64Put(actual_blocks as uint64, 24, b);
     }
 
     static method decode(b: Bytes, ghost sb0: SuperBlock) returns (sb: SuperBlock)
@@ -101,8 +101,8 @@ module FsKinds {
       }
       var inode_blocks := Marshal.UInt64Decode(b, 8, sb0.info.inode_blocks as uint64);
       var data_bitmaps := Marshal.UInt64Decode(b, 16, sb0.info.data_bitmaps as uint64);
-      var disk_size := Marshal.UInt64Decode(b, 24, sb0.disk_size);
-      return SuperBlock(Super(inode_blocks as nat, data_bitmaps as nat), disk_size);
+      var actual_blocks := Marshal.UInt64Decode(b, 24, sb0.actual_blocks);
+      return SuperBlock(Super(inode_blocks as nat, data_bitmaps as nat), actual_blocks);
     }
   }
 
@@ -134,6 +134,8 @@ module FsKinds {
   lemma NumBlocks_upper_bound()
     ensures super.disk_size < 200_000
   {}
+
+  const SuperBlkAddr: Addr := Addr(Super.block_addr, 0);
 
   function method InodeBlk(ino: Ino): (bn':Blkno)
     ensures InodeBlk?(bn')
@@ -271,6 +273,16 @@ module FsKinds {
   lemma fs_kinds_valid()
     ensures kindsValid(fs_kinds)
   {}
+
+  lemma super_block_inbounds(jrnl: Jrnl)
+    requires jrnl.Valid()
+    requires jrnl.kinds == fs_kinds
+    ensures SuperBlkAddr in jrnl.data && jrnl.size(SuperBlkAddr) == 4096*8
+  {
+    assert kindSize(KindBlock) == 4096*8;
+    jrnl.in_domain(SuperBlkAddr);
+    jrnl.has_size(SuperBlkAddr);
+  }
 
   lemma blkno_bit_inbounds(jrnl: Jrnl)
     requires jrnl.Valid()
